12AssemblyCode/AssemblyCode.thy
@@ -2,51 +2,116 @@ theory AssemblyCode
   imports "../00Utils/Iteration" "../00Utils/Environment"
 begin
 
-datatype register = Hp | Env | Vals | Stk | Acc
+section \<open>Assembly Code\<close>
 
-datatype move_src = Reg register | Con nat 
+text \<open>With our transitions reduced to simple function updates and arithmetic operations, we are 
+ready to take the final step and move to a low-level, machine-like execution model. For the first 
+time, we have choices in our development: we could use a real processor (any of a number of real 
+processors, for that matter) or define our own. For simplicity - and because our correctness proof 
+relies on a truly unbounded memory, indexed by unbounded naturals, which no real machine has - we 
+define a simple machine based in a general way on Nisan and Schocken's tutorial HACK processor [4].\<close>
+
+text \<open>Our processor has five registers, one each for the stack pointers for the value heap, 
+environment heap, value stack, and callstack, and one as an accumulator. It also has a special 
+register for the code-pointer, and an infinite natural-indexed memory.\<close>
+
+text \<open>For this stage, in order to ease the already quite-involved conversion, we imbue the processor 
+with a little more structure. We tag each memory cell and the accumulator register with a memory 
+segment, to say what kind of pointer lives in it. (\<open>Acc\<close> stands for non-pointers.) We also keep our 
+four memory segments separate in the memory map; this leaves us with an extra segment for \<open>Acc\<close> but
+it will remain unused and we will arrange to allocate no space for it in the final memory layout.\<close>
+
+datatype memseg = Hp | Env | Vals | Stk | Acc
+
+datatype assm_state = S\<^sub>a "memseg \<Rightarrow> nat \<Rightarrow> memseg \<times> nat" "memseg \<Rightarrow> nat" memseg nat
+
+text \<open>We have a small, RISC-like (not to say minimalistic) set of operations on the processor. We 
+can do simple arithmetic on the registers; we can move values between registers, and load and store 
+into memory; and we can jump, to a static address or indirectly to an address in a register. We will
+not need all of even this small set of functionality (we never add or subtract a non-constant, or 
+make a direct jump, for instance) but we include it to make the processor plausible and for future 
+expansion of the source language.\<close>
+
+text \<open>In our assembler, we allow ourselves some liberties with the opcodes. The operate-on-register/
+operate-on-constant opcodes are collapsed into a single assembly operation; and the move/load/store 
+operations are likewise reduced to a single \<open>AMov\<close> operation with a number of addressing modes.\<close>
+
+datatype addr_mode = Reg memseg | Con nat
+
+datatype move_src = Reg memseg | Con nat | Mem memseg
 
 datatype assm = 
-  AGet register
-  | APut register move_src
-  | ASub register nat
-  | AAdd register nat
+  APut memseg move_src
+  | ASub memseg nat
+  | AAdd memseg nat
   | AJmp
 
-datatype assm_state = 
-  AS "register \<Rightarrow> nat \<Rightarrow> register \<times> nat" "register \<Rightarrow> nat" register nat
-
-fun mem_upd :: "(register \<Rightarrow> nat \<Rightarrow> register \<times> nat) \<Rightarrow> register \<Rightarrow> nat \<Rightarrow> register \<times> nat \<Rightarrow> 
-    register \<Rightarrow> nat \<Rightarrow> register \<times> nat" where
+fun mem_upd :: "(memseg \<Rightarrow> nat \<Rightarrow> memseg \<times> nat) \<Rightarrow> memseg \<Rightarrow> nat \<Rightarrow> memseg \<times> nat \<Rightarrow> 
+    memseg \<Rightarrow> nat \<Rightarrow> memseg \<times> nat" where
   "mem_upd mem m mp k m' x = (if m = m' \<and> mp = x then k else mem m' x)"
 
-abbreviation reg_merge :: "register \<Rightarrow> register \<Rightarrow> register" where
+inductive evala :: "assm list \<Rightarrow> assm_state \<Rightarrow> assm_state \<Rightarrow> bool" (infix "\<tturnstile> _ \<leadsto>\<^sub>a" 50) where
+  eva_movr [simp]: "lookup cd pc = Some (APut Acc (Reg r)) \<Longrightarrow> r \<noteq> Acc \<Longrightarrow>
+    cd \<tturnstile> S\<^sub>a mem ps act (Suc pc) \<leadsto>\<^sub>a S\<^sub>a mem (ps(Acc := ps r)) r pc"
+| eva_mova [simp]: "lookup cd pc = Some (APut Acc (Reg Acc)) \<Longrightarrow> 
+    cd \<tturnstile> S\<^sub>a mem ps act (Suc pc) \<leadsto>\<^sub>a S\<^sub>a mem ps act pc"
+| eva_movk [simp]: "lookup cd pc = Some (APut Acc (Con k)) \<Longrightarrow> 
+    cd \<tturnstile> S\<^sub>a mem ps act (Suc pc) \<leadsto>\<^sub>a S\<^sub>a mem (ps(Acc := k)) Acc pc"
+| eva_lod [simp]: "lookup cd pc = Some (APut Acc (Mem r')) \<Longrightarrow> mem r' (ps r') = (t, b) \<Longrightarrow> r' \<noteq> Acc \<Longrightarrow>
+    cd \<tturnstile> S\<^sub>a mem ps act (Suc pc) \<leadsto>\<^sub>a S\<^sub>a mem (ps(Acc := b)) t pc"
+| eva_loda [simp]: "lookup cd pc = Some (APut Acc (Mem Acc)) \<Longrightarrow> mem act (ps Acc) = (t, b) \<Longrightarrow> act \<noteq> Acc \<Longrightarrow>
+    cd \<tturnstile> S\<^sub>a mem ps act (Suc pc) \<leadsto>\<^sub>a S\<^sub>a mem (ps(Acc := b)) t pc"
+| eva_putr [simp]: "lookup cd pc = Some (APut r (Reg r')) \<Longrightarrow> r \<noteq> Acc \<Longrightarrow> r' \<noteq> Acc \<Longrightarrow>
+    cd \<tturnstile> S\<^sub>a mem ps act (Suc pc) \<leadsto>\<^sub>a S\<^sub>a (mem_upd mem r (ps r) (r', ps r')) ps act pc"
+| eva_puta [simp]: "lookup cd pc = Some (APut r (Reg Acc)) \<Longrightarrow> r \<noteq> Acc \<Longrightarrow>
+    cd \<tturnstile> S\<^sub>a mem ps act (Suc pc) \<leadsto>\<^sub>a S\<^sub>a (mem_upd mem r (ps r) (act, ps Acc)) ps act pc"
+| eva_putk [simp]: "lookup cd pc = Some (APut r (Con k)) \<Longrightarrow> r \<noteq> Acc \<Longrightarrow>
+    cd \<tturnstile> S\<^sub>a mem ps act (Suc pc) \<leadsto>\<^sub>a S\<^sub>a (mem_upd mem r (ps r) (Acc, k)) ps act pc"
+| eva_get [simp]: "lookup cd pc = Some (APut r (Mem r')) \<Longrightarrow> mem r' (ps r') = (r, b) \<Longrightarrow> 
+      r' \<noteq> Acc \<Longrightarrow> r \<noteq> Acc \<Longrightarrow>
+    cd \<tturnstile> S\<^sub>a mem ps act (Suc pc) \<leadsto>\<^sub>a S\<^sub>a mem (ps(r := b)) act pc"
+| eva_geta [simp]: "lookup cd pc = Some (APut r (Mem Acc)) \<Longrightarrow> mem act (ps Acc) = (r, b) \<Longrightarrow> 
+      r \<noteq> Acc \<Longrightarrow> act \<noteq> Acc \<Longrightarrow>
+    cd \<tturnstile> S\<^sub>a mem ps act (Suc pc) \<leadsto>\<^sub>a S\<^sub>a mem (ps(r := b)) act pc"
+| eva_suba [simp]: "lookup cd pc = Some (ASub Acc k) \<Longrightarrow> ps Acc \<ge> k \<Longrightarrow> act \<noteq> Acc \<Longrightarrow>
+    cd \<tturnstile> S\<^sub>a mem ps act (Suc pc) \<leadsto>\<^sub>a S\<^sub>a mem (ps(Acc := ps Acc - k)) act pc"
+| eva_sub [simp]: "lookup cd pc = Some (ASub r k) \<Longrightarrow> ps r \<ge> k \<Longrightarrow> r \<noteq> Acc \<Longrightarrow>
+    cd \<tturnstile> S\<^sub>a mem ps act (Suc pc) \<leadsto>\<^sub>a S\<^sub>a mem (ps(r := ps r - k)) act pc"
+| eva_add [simp]: "lookup cd pc = Some (AAdd r k) \<Longrightarrow> r \<noteq> Acc \<Longrightarrow>
+    cd \<tturnstile> S\<^sub>a mem ps act (Suc pc) \<leadsto>\<^sub>a S\<^sub>a mem (ps(r := ps r + k)) act pc"
+| eva_adda [simp]: "lookup cd pc = Some (AAdd Acc k) \<Longrightarrow> act \<noteq> Acc \<Longrightarrow>
+    cd \<tturnstile> S\<^sub>a mem ps act (Suc pc) \<leadsto>\<^sub>a S\<^sub>a mem (ps(Acc := ps Acc + k)) act pc"
+| eva_jmp [simp]: "lookup cd pc = Some AJmp \<Longrightarrow> 
+    cd \<tturnstile> S\<^sub>a mem ps Acc (Suc pc) \<leadsto>\<^sub>a S\<^sub>a mem (ps(Acc := 0)) Acc (ps Acc)"
+
+abbreviation reg_merge :: "memseg \<Rightarrow> memseg \<Rightarrow> memseg" where
   "reg_merge a b \<equiv> (if a = Acc then b else a)"
 
-fun assm_step :: "(register \<Rightarrow> nat \<Rightarrow> register \<times> nat) \<Rightarrow> (register \<Rightarrow> nat) \<Rightarrow> register \<Rightarrow> nat \<Rightarrow> 
+fun assm_step :: "(memseg \<Rightarrow> nat \<Rightarrow> memseg \<times> nat) \<Rightarrow> (memseg \<Rightarrow> nat) \<Rightarrow> memseg \<Rightarrow> nat \<Rightarrow> 
     assm \<rightharpoonup> assm_state" where
-  "assm_step mem ps act pc (AGet r) = 
-    (if r = Acc \<and> act = Acc then None
-     else case mem (reg_merge r act) (ps r) of
-       (t, b) \<Rightarrow> Some (AS mem (ps(Acc := b)) t pc))"
-| "assm_step mem ps act pc (APut Acc (Reg r')) = 
-    Some (AS mem (ps(Acc := ps r')) (reg_merge r' act) pc)"
-| "assm_step mem ps act pc (APut Acc (Con k)) = Some (AS mem (ps(Acc := k)) Acc pc)"
+  "assm_step mem ps act pc (APut Acc (Reg r')) = 
+    Some (S\<^sub>a mem (ps(Acc := ps r')) (reg_merge r' act) pc)"
+| "assm_step mem ps act pc (APut Acc (Con k)) = 
+    Some (S\<^sub>a mem (ps(Acc := k)) Acc pc)"
+| "assm_step mem ps act pc (APut Acc (Mem r')) = (case mem (reg_merge r' act) (ps r') of
+     (t, b) \<Rightarrow> if r' \<noteq> Acc \<or> act \<noteq> Acc then Some (S\<^sub>a mem (ps(Acc := b)) t pc) else None)"
 | "assm_step mem ps act pc (APut r (Reg r')) = 
-    Some (AS (mem_upd mem r (ps r) (reg_merge r' act, ps r')) ps act pc)"
+    Some (S\<^sub>a (mem_upd mem r (ps r) (reg_merge r' act, ps r')) ps act pc)"
 | "assm_step mem ps act pc (APut r (Con k)) = 
-    Some (AS (mem_upd mem r (ps r) (Acc, k)) ps act pc)"
+    Some (S\<^sub>a (mem_upd mem r (ps r) (Acc, k)) ps act pc)"
+| "assm_step mem ps act pc (APut r (Mem r')) = (case mem (reg_merge r' act) (ps r') of
+     (t, b) \<Rightarrow> if t = r \<and> (r' \<noteq> Acc \<or> act \<noteq> Acc) then Some (S\<^sub>a mem (ps(r := b)) act pc) else None)"
 | "assm_step mem ps act pc (ASub r k) = 
     (if ps r < k \<or> (r = Acc \<and> act = Acc) then None 
-     else Some (AS mem (ps(r := ps r - k)) act pc))"
+     else Some (S\<^sub>a mem (ps(r := ps r - k)) act pc))"
 | "assm_step mem ps act pc (AAdd r k) = 
     (if r = Acc \<and> act = Acc then None 
-     else Some (AS mem (ps(r := ps r + k)) act pc))"
+     else Some (S\<^sub>a mem (ps(r := ps r + k)) act pc))"
 | "assm_step mem ps act pc AJmp = 
-    (if act = Acc then Some (AS mem (ps(Acc := 0)) Acc (ps Acc)) else None)"
+    (if act = Acc then Some (S\<^sub>a mem (ps(Acc := 0)) Acc (ps Acc)) else None)"
 
 fun alg_evala :: "assm list \<Rightarrow> assm_state \<rightharpoonup> assm_state" (infix "\<tturnstile>\<^sub>a" 50) where
-  "cd \<tturnstile>\<^sub>a AS mem ps act pc = (case pc of
+  "cd \<tturnstile>\<^sub>a S\<^sub>a mem ps act pc = (case pc of
       0 \<Rightarrow> None
     | Suc pc \<Rightarrow> Option.bind (lookup cd pc) (assm_step mem ps act pc))"
 
@@ -54,60 +119,32 @@ primrec iter_evala :: "assm list \<Rightarrow> nat \<Rightarrow> assm_state \<ri
   "iter_evala cd 0 \<Sigma> = Some \<Sigma>"
 | "iter_evala cd (Suc x) \<Sigma> = Option.bind (cd \<tturnstile>\<^sub>a \<Sigma>) (iter_evala cd x)"
 
-inductive evala :: "assm list \<Rightarrow> assm_state \<Rightarrow> assm_state \<Rightarrow> bool" (infix "\<tturnstile> _ \<leadsto>\<^sub>a" 50) where
-  eva_movr [simp]: "lookup cd pc = Some (APut Acc (Reg r)) \<Longrightarrow> r \<noteq> Acc \<Longrightarrow>
-    cd \<tturnstile> AS mem ps act (Suc pc) \<leadsto>\<^sub>a AS mem (ps(Acc := ps r)) r pc"
-| eva_mova [simp]: "lookup cd pc = Some (APut Acc (Reg Acc)) \<Longrightarrow> 
-    cd \<tturnstile> AS mem ps act (Suc pc) \<leadsto>\<^sub>a AS mem ps act pc"
-| eva_movk [simp]: "lookup cd pc = Some (APut Acc (Con k)) \<Longrightarrow> 
-    cd \<tturnstile> AS mem ps act (Suc pc) \<leadsto>\<^sub>a AS mem (ps(Acc := k)) Acc pc"
-| eva_get [simp]: "lookup cd pc = Some (AGet r) \<Longrightarrow> mem r (ps r) = (t, b) \<Longrightarrow> r \<noteq> Acc \<Longrightarrow>
-    cd \<tturnstile> AS mem ps act (Suc pc) \<leadsto>\<^sub>a AS mem (ps(Acc := b)) t pc"
-| eva_geta [simp]: "lookup cd pc = Some (AGet Acc) \<Longrightarrow> mem act (ps Acc) = (t, b) \<Longrightarrow> act \<noteq> Acc \<Longrightarrow>
-    cd \<tturnstile> AS mem ps act (Suc pc) \<leadsto>\<^sub>a AS mem (ps(Acc := b)) t pc"
-| eva_putr [simp]: "lookup cd pc = Some (APut r (Reg r')) \<Longrightarrow> r \<noteq> Acc \<Longrightarrow> r' \<noteq> Acc \<Longrightarrow>
-    cd \<tturnstile> AS mem ps act (Suc pc) \<leadsto>\<^sub>a AS (mem_upd mem r (ps r) (r', ps r')) ps act pc"
-| eva_puta [simp]: "lookup cd pc = Some (APut r (Reg Acc)) \<Longrightarrow> r \<noteq> Acc \<Longrightarrow>
-    cd \<tturnstile> AS mem ps act (Suc pc) \<leadsto>\<^sub>a AS (mem_upd mem r (ps r) (act, ps Acc)) ps act pc"
-| eva_putk [simp]: "lookup cd pc = Some (APut r (Con k)) \<Longrightarrow> r \<noteq> Acc \<Longrightarrow>
-    cd \<tturnstile> AS mem ps act (Suc pc) \<leadsto>\<^sub>a AS (mem_upd mem r (ps r) (Acc, k)) ps act pc"
-| eva_suba [simp]: "lookup cd pc = Some (ASub Acc k) \<Longrightarrow> ps Acc \<ge> k \<Longrightarrow> act \<noteq> Acc \<Longrightarrow>
-    cd \<tturnstile> AS mem ps act (Suc pc) \<leadsto>\<^sub>a AS mem (ps(Acc := ps Acc - k)) act pc"
-| eva_sub [simp]: "lookup cd pc = Some (ASub r k) \<Longrightarrow> ps r \<ge> k \<Longrightarrow> r \<noteq> Acc \<Longrightarrow>
-    cd \<tturnstile> AS mem ps act (Suc pc) \<leadsto>\<^sub>a AS mem (ps(r := ps r - k)) act pc"
-| eva_add [simp]: "lookup cd pc = Some (AAdd r k) \<Longrightarrow> r \<noteq> Acc \<Longrightarrow>
-    cd \<tturnstile> AS mem ps act (Suc pc) \<leadsto>\<^sub>a AS mem (ps(r := ps r + k)) act pc"
-| eva_adda [simp]: "lookup cd pc = Some (AAdd Acc k) \<Longrightarrow> act \<noteq> Acc \<Longrightarrow>
-    cd \<tturnstile> AS mem ps act (Suc pc) \<leadsto>\<^sub>a AS mem (ps(Acc := ps Acc + k)) act pc"
-| eva_jmp [simp]: "lookup cd pc = Some AJmp \<Longrightarrow> 
-    cd \<tturnstile> AS mem ps Acc (Suc pc) \<leadsto>\<^sub>a AS mem (ps(Acc := 0)) Acc (ps Acc)"
-
-lemma [simp]: "mem_upd (case_register h e vs sh a) Hp x y = case_register (h(x := y)) e vs sh a"
+lemma [simp]: "mem_upd (case_memseg h e vs sh a) Hp x y = case_memseg (h(x := y)) e vs sh a"
 proof (rule, rule)
   fix m n
-  show "mem_upd (case_register h e vs sh a) Hp x y m n = case_register (h(x := y)) e vs sh a m n"
-    by (induction m) (simp_all split: register.splits)
+  show "mem_upd (case_memseg h e vs sh a) Hp x y m n = case_memseg (h(x := y)) e vs sh a m n"
+    by (induction m) (simp_all split: memseg.splits)
 qed
 
-lemma [simp]: "mem_upd (case_register h e vs sh a) Env x y = case_register h (e(x := y)) vs sh a"
+lemma [simp]: "mem_upd (case_memseg h e vs sh a) Env x y = case_memseg h (e(x := y)) vs sh a"
 proof (rule, rule)
   fix m n
-  show "mem_upd (case_register h e vs sh a) Env x y m n = case_register h (e(x := y)) vs sh a m n"
-    by (induction m) (simp_all split: register.splits)
+  show "mem_upd (case_memseg h e vs sh a) Env x y m n = case_memseg h (e(x := y)) vs sh a m n"
+    by (induction m) (simp_all split: memseg.splits)
 qed
 
-lemma [simp]: "mem_upd (case_register h e vs sh a) Vals x y = case_register h e (vs(x := y)) sh a"
+lemma [simp]: "mem_upd (case_memseg h e vs sh a) Vals x y = case_memseg h e (vs(x := y)) sh a"
 proof (rule, rule)
   fix m n
-  show "mem_upd (case_register h e vs sh a) Vals x y m n = case_register h e (vs(x := y)) sh a m n"
-    by (induction m) (simp_all split: register.splits)
+  show "mem_upd (case_memseg h e vs sh a) Vals x y m n = case_memseg h e (vs(x := y)) sh a m n"
+    by (induction m) (simp_all split: memseg.splits)
 qed
 
-lemma [simp]: "mem_upd (case_register h e vs sh a) Stk x y = case_register h e vs (sh(x := y)) a"
+lemma [simp]: "mem_upd (case_memseg h e vs sh a) Stk x y = case_memseg h e vs (sh(x := y)) a"
 proof (rule, rule)
   fix m n
-  show "mem_upd (case_register h e vs sh a) Stk x y m n = case_register h e vs (sh(x := y)) a m n"
-    by (induction m) (simp_all split: register.splits)
+  show "mem_upd (case_memseg h e vs sh a) Stk x y m n = case_memseg h e vs (sh(x := y)) a m n"
+    by (induction m) (simp_all split: memseg.splits)
 qed
 
 lemma iter_evala_combine [simp]: "iter_evala cd n \<Sigma> = Some \<Sigma>' \<Longrightarrow> 
@@ -118,21 +155,21 @@ proof (induction n arbitrary: \<Sigma>)
 qed simp_all
 
 lemma assm_step_equiv: "(Option.bind (lookup cd pc) (assm_step mem ps act pc) = Some \<Sigma>) \<Longrightarrow>
-  (cd \<tturnstile> AS mem ps act (Suc pc) \<leadsto>\<^sub>a \<Sigma>)"
+  (cd \<tturnstile> S\<^sub>a mem ps act (Suc pc) \<leadsto>\<^sub>a \<Sigma>)"
 proof (cases "lookup cd pc")
   case (Some op)
   moreover assume "Option.bind (lookup cd pc) (assm_step mem ps act pc) = Some \<Sigma>"
   ultimately show ?thesis 
   proof (induction mem ps act pc op rule: assm_step.induct)
-    case (6 mem ps act pc r k)
+    case (7 mem ps act pc r k)
     then show ?case by (cases r) (auto split: if_splits)
   next
-    case (7 mem ps act pc r k)
+    case (8 mem ps act pc r k)
     then show ?case by (cases r) (auto split: if_splits)
   qed (auto split: if_splits prod.splits option.splits)
 qed simp_all
 
-lemma alg_evala_equiv: "cd \<tturnstile>\<^sub>a \<Sigma> = Some \<Sigma>' = (cd \<tturnstile> \<Sigma> \<leadsto>\<^sub>a \<Sigma>')"
+lemma alg_evala_equiv: "(cd \<tturnstile> \<Sigma> \<leadsto>\<^sub>a \<Sigma>') = (cd \<tturnstile>\<^sub>a \<Sigma> = Some \<Sigma>')"
 proof
   show "cd \<tturnstile>\<^sub>a \<Sigma> = Some \<Sigma>' \<Longrightarrow> cd \<tturnstile> \<Sigma> \<leadsto>\<^sub>a \<Sigma>'"
     by (induction \<Sigma>) (auto simp add: assm_step_equiv split: nat.splits)
@@ -146,10 +183,16 @@ proof
   next
     case (eva_putk cd pc r k mem ps act)
     thus ?case by (induction r) simp_all
+  next
+    case (eva_get cd pc r r' mem ps b act)
+    thus ?case by (induction r) simp_all
+  next
+    case (eva_geta cd pc r mem act ps b)
+    thus ?case by (induction r) simp_all
   qed simp_all
 qed
 
-lemma iter_evala_equiv: "(\<exists>n. iter_evala cd n \<Sigma> = Some \<Sigma>') = iter (\<tturnstile> cd \<leadsto>\<^sub>a) \<Sigma> \<Sigma>'"
+lemma iter_evala_equiv: "iter (\<tturnstile> cd \<leadsto>\<^sub>a) \<Sigma> \<Sigma>' = (\<exists>n. iter_evala cd n \<Sigma> = Some \<Sigma>')"
 proof
   assume "\<exists>n. iter_evala cd n \<Sigma> = Some \<Sigma>'"
   then obtain n where "iter_evala cd n \<Sigma> = Some \<Sigma>'" by fastforce
@@ -174,12 +217,6 @@ next
 qed
 
 theorem determinisma: "cd \<tturnstile> \<Sigma> \<leadsto>\<^sub>a \<Sigma>' \<Longrightarrow> cd \<tturnstile> \<Sigma> \<leadsto>\<^sub>a \<Sigma>'' \<Longrightarrow> \<Sigma>' = \<Sigma>''"
-proof -
-  assume "cd \<tturnstile> \<Sigma> \<leadsto>\<^sub>a \<Sigma>'" 
-  hence X: "cd \<tturnstile>\<^sub>a \<Sigma> = Some \<Sigma>'" by (simp add: alg_evala_equiv)
-  assume "cd \<tturnstile> \<Sigma> \<leadsto>\<^sub>a \<Sigma>''"
-  hence "cd \<tturnstile>\<^sub>a \<Sigma> = Some \<Sigma>''" by (simp add: alg_evala_equiv)
-  with X show "\<Sigma>' = \<Sigma>''" by simp
-qed
+  by (simp add: alg_evala_equiv)
 
 end
