13MachineCode/Disassemble.thy
@@ -2,14 +2,14 @@ theory Disassemble
   imports MachineCode "../12AssemblyCode/AssemblyCode"
 begin
 
-primrec register_map :: "register \<Rightarrow> reg" where
+primrec register_map :: "memseg \<Rightarrow> reg" where
   "register_map Hp = R1"
 | "register_map Env = R2"
 | "register_map Vals = R3"
 | "register_map Stk = R4"
 | "register_map Acc = R5"
 
-primrec register_offset :: "register \<Rightarrow> nat" where
+primrec register_offset :: "memseg \<Rightarrow> nat" where
   "register_offset Hp = 0"
 | "register_offset Env = 1"
 | "register_offset Vals = 2"
@@ -19,15 +19,16 @@ primrec register_offset :: "register \<Rightarrow> nat" where
 primrec pseudoreg_size :: "move_src \<Rightarrow> nat" where
   "pseudoreg_size (Reg r) = (if r = Acc then 1 else 4)"
 | "pseudoreg_size (Con k) = 1"
+| "pseudoreg_size (Mem r) = 1"
 
-primrec pseudoreg_map :: "register \<times> nat \<Rightarrow> nat" where
+primrec pseudoreg_map :: "memseg \<times> nat \<Rightarrow> nat" where
   "pseudoreg_map (r, x) = (if r = Acc then x else 4 * x + register_offset r)"
 
 fun disassemble' :: "assm \<Rightarrow> mach" where
-  "disassemble' (AGet r) = LOD R5 (register_map r)"
-| "disassemble' (APut r (Reg r')) = 
+  "disassemble' (APut r (Reg r')) = 
     (if r = Acc then MOV R5 (register_map r') else STO (register_map r) (register_map r'))"
 | "disassemble' (APut r (Con k)) = (if r = Acc then LDI R5 k else STI (register_map r) k)"
+| "disassemble' (APut r (Mem r')) = LOD (register_map r) (register_map r')"
 | "disassemble' (ASub r k) = SUB (register_map r) (4 * k)"
 | "disassemble' (AAdd r k) = ADD (register_map r) (4 * k)"
 | "disassemble' AJmp = JMP R5"
@@ -35,17 +36,17 @@ fun disassemble' :: "assm \<Rightarrow> mach" where
 definition disassemble :: "assm list \<Rightarrow> mach list" where
   "disassemble cd = map disassemble' cd"
 
-fun unmap_mem' :: "nat \<Rightarrow> register \<times> nat" where
+fun unmap_mem' :: "nat \<Rightarrow> memseg \<times> nat" where
   "unmap_mem' 0 = (Hp, 0)" 
 | "unmap_mem' (Suc 0) = (Env, 0)"
 | "unmap_mem' (Suc (Suc 0)) = (Vals, 0)"
 | "unmap_mem' (Suc (Suc (Suc 0))) = (Stk, 0)"
 | "unmap_mem' (Suc (Suc (Suc (Suc x)))) = (case unmap_mem' x of (a, b) \<Rightarrow> (a, Suc b))"
 
-definition unmap_mem :: "(register \<Rightarrow> nat \<Rightarrow> register \<times> nat) \<Rightarrow> nat \<Rightarrow> nat" where
+definition unmap_mem :: "(memseg \<Rightarrow> nat \<Rightarrow> memseg \<times> nat) \<Rightarrow> nat \<Rightarrow> nat" where
   "unmap_mem m x = (case unmap_mem' x of (r, p) \<Rightarrow> pseudoreg_map (m r p))"
 
-primrec inv_register_map :: "(register \<Rightarrow> nat) \<Rightarrow> register \<Rightarrow> reg \<Rightarrow> nat" where
+primrec inv_register_map :: "(memseg \<Rightarrow> nat) \<Rightarrow> memseg \<Rightarrow> reg \<Rightarrow> nat" where
   "inv_register_map rs t R1 = rs Hp * 4"
 | "inv_register_map rs t R2 = rs Env * 4 + 1"
 | "inv_register_map rs t R3 = rs Vals * 4 + 2"
@@ -53,10 +54,10 @@ primrec inv_register_map :: "(register \<Rightarrow> nat) \<Rightarrow> register
 | "inv_register_map rs t R5 = pseudoreg_map (t, rs Acc)"
 
 primrec disassemble_state :: "assm_state \<Rightarrow> mach_state" where
-  "disassemble_state (AS mem rs t pc) = MS (inv_register_map rs t) (unmap_mem mem) pc"
+  "disassemble_state (S\<^sub>a mem rs t pc) = MS (inv_register_map rs t) (unmap_mem mem) pc"
 
 primrec dissassembleable :: "assm_state \<Rightarrow> nat \<Rightarrow> bool" where
-  "dissassembleable (AS mem rs t pc) lcd = (pc < lcd)"
+  "dissassembleable (S\<^sub>a mem rs t pc) lcd = (pc < lcd)"
 
 lemma [dest]: "R1 = register_map r \<Longrightarrow> r = Hp"
   by (induction r) simp_all
@@ -74,6 +75,18 @@ lemma [dest]: "R5 = register_map r \<Longrightarrow> r = Acc"
   by (induction r) simp_all
 
 lemma unmap_times_4 [simp]: "unmap_mem' (4 * k) = (Hp, k)"
+  by (induction k) (simp_all add: numeral_def)
+
+lemma [simp]: "unmap_mem' (k * 4) = (Hp, k)"
+  by (induction k) (simp_all add: numeral_def)
+
+lemma [simp]: "unmap_mem' (Suc (k * 4)) = (Env, k)"
+  by (induction k) (simp_all add: numeral_def)
+
+lemma [simp]: "unmap_mem' (Suc (Suc (k * 4))) = (Vals, k)"
+  by (induction k) (simp_all add: numeral_def)
+
+lemma [simp]: "unmap_mem' (k * 4 + 3) = (Stk, k)"
   by (induction k) (simp_all add: numeral_def)
 
 lemma [simp]: "unmap_mem' p = (a, b) \<Longrightarrow> unmap_mem' (4 + p) = (a, Suc b)"
@@ -106,6 +119,9 @@ proof -
   thus ?thesis by simp
 qed
 
+lemma [simp]: "r \<noteq> Acc \<Longrightarrow> unmap_mem' (inv_register_map ps act (register_map r)) = (r, ps r)"
+  by (induction r) simp_all
+
 lemma inv_reg_map_reg: "r \<noteq> Acc \<Longrightarrow>
   (inv_register_map ps act)(R5 := inv_register_map ps act (register_map r)) = 
     inv_register_map (ps(Acc := ps r)) r"
@@ -130,18 +146,6 @@ qed
 lemma [simp]: "(inv_register_map ps act)
     (R5 := if act = Acc then ps Acc else 4 * ps Acc + register_offset act) = inv_register_map ps act"
   by auto
-
-lemma [simp]: "unmap_mem' (k * 4) = (Hp, k)"
-  by (induction k) (simp_all add: numeral_def)
-
-lemma [simp]: "unmap_mem' (Suc (k * 4)) = (Env, k)"
-  by (induction k) (simp_all add: numeral_def)
-
-lemma [simp]: "unmap_mem' (Suc (Suc (k * 4))) = (Vals, k)"
-  by (induction k) (simp_all add: numeral_def)
-
-lemma [simp]: "unmap_mem' (k * 4 + 3) = (Stk, k)"
-  by (induction k) (simp_all add: numeral_def)
 
 lemma [simp]: "m \<noteq> Acc \<Longrightarrow> unmap_mem' (4 * k + register_offset m) = (m, k)"
 proof (induction k)
@@ -265,6 +269,46 @@ proof
       by (induction x) (auto simp add: unmap_mem_def)
 qed
 
+lemma [simp]: "mem act (ps Acc) = (r, b) \<Longrightarrow> r \<noteq> Acc \<Longrightarrow> act \<noteq> Acc \<Longrightarrow>
+  ((inv_register_map ps act)(register_map r := unmap_mem mem (4 * ps Acc + register_offset act))) =
+    (inv_register_map (ps(r := b)) act)"
+proof 
+  fix x
+  assume "mem act (ps Acc) = (r, b)" and "act \<noteq> Acc" and "r \<noteq> Acc"
+  thus "((inv_register_map ps act)
+    (register_map r := unmap_mem mem (4 * ps Acc + register_offset act))) x =
+      (inv_register_map (ps(r := b)) act) x"
+    by (induction x) (auto simp add: unmap_mem_def)
+qed
+
+lemma [simp]: "mem r' (ps r') = (r, b) \<Longrightarrow> r' \<noteq> Acc \<Longrightarrow> r \<noteq> Acc \<Longrightarrow>
+  ((inv_register_map ps act) 
+    (register_map r := unmap_mem mem (inv_register_map ps act (register_map r')))) =
+      (inv_register_map (ps(r := b)) act)"
+proof 
+  fix x
+  assume "mem r' (ps r') = (r, b)" and "r' \<noteq> Acc" and "r \<noteq> Acc"
+  thus "((inv_register_map ps act)
+    (register_map r := unmap_mem mem (inv_register_map ps act (register_map r')))) x =
+      (inv_register_map (ps(r := b)) act) x"
+  proof (induction x)
+    case R1
+    thus ?case by (induction r) (simp_all add: unmap_mem_def)
+  next
+    case R2
+    thus ?case by (induction r) (simp_all add: unmap_mem_def)
+  next
+    case R3
+    thus ?case by (induction r) (simp_all add: unmap_mem_def)
+  next
+    case R4
+    thus ?case by (induction r) (simp_all add: unmap_mem_def)
+  next
+    case R5
+    thus ?case by (induction r) (simp_all add: unmap_mem_def)
+  qed 
+qed
+
 lemma [simp]: "(inv_register_map ps act)(R5 := pseudoreg_map (act, ps Acc)) = inv_register_map ps act"
   by auto
 
@@ -288,7 +332,6 @@ next
   hence "disassemble cd \<tturnstile> MS (inv_register_map ps act) (unmap_mem mem) (Suc pc) \<leadsto>\<^sub>m 
     MS ((inv_register_map ps act)(R5 := inv_register_map ps act R5)) (unmap_mem mem) pc" 
       by (metis evm_mov)
-
   hence "disassemble cd \<tturnstile> MS (inv_register_map ps act) (unmap_mem mem) (Suc pc) \<leadsto>\<^sub>m
     MS (inv_register_map ps act) (unmap_mem mem) pc" by simp
   thus ?case by simp
@@ -298,19 +341,33 @@ next
     MS ((inv_register_map ps act)(R5 := k)) (unmap_mem mem) pc" by simp
   thus ?case by (simp add: inv_reg_map_none)
 next
-  case (eva_geta cd pc mem r ps t b) 
-  hence "disassemble cd ! pc = LOD R5 R5" by simp
-  hence "disassemble cd \<tturnstile> MS (inv_register_map ps r) (unmap_mem mem) (Suc pc) \<leadsto>\<^sub>m 
-    MS ((inv_register_map ps r)(R5 := unmap_mem mem (inv_register_map ps r R5))) 
+  case (eva_lod cd pc r' mem ps t b act)
+  hence "disassemble cd ! pc = LOD R5 (register_map r')" by simp
+  hence "disassemble cd \<tturnstile> MS (inv_register_map ps act) (unmap_mem mem) (Suc pc) \<leadsto>\<^sub>m 
+    MS ((inv_register_map ps act)(R5 := unmap_mem mem (inv_register_map ps act (register_map r')))) 
       (unmap_mem mem) pc" by (metis evm_lod)
-  with eva_geta(2, 3) show ?case by simp
+  with eva_lod(2, 3) show ?case by simp
 next
-  case (eva_get cd pc r mem ps t b act)
-  hence "disassemble cd ! pc = LOD R5 (register_map r)" by simp
+  case (eva_loda cd pc mem act ps t b)  
+  hence "disassemble cd ! pc = LOD R5 R5" by simp
+  hence "disassemble cd \<tturnstile> MS (inv_register_map ps act) (unmap_mem mem) (Suc pc) \<leadsto>\<^sub>m 
+    MS ((inv_register_map ps act)(R5 := unmap_mem mem (inv_register_map ps act R5))) 
+      (unmap_mem mem) pc" by (metis evm_lod)
+  with eva_loda(2, 3) show ?case by simp
+next
+  case (eva_geta cd pc r mem act ps b) 
+  hence "disassemble cd ! pc = LOD (register_map r) R5" by simp
+  hence "disassemble cd \<tturnstile> MS (inv_register_map ps act) (unmap_mem mem) (Suc pc) \<leadsto>\<^sub>m 
+    MS ((inv_register_map ps act)(register_map r := unmap_mem mem (inv_register_map ps act R5))) 
+      (unmap_mem mem) pc" by (metis evm_lod)
+  with eva_geta(2, 3, 4) show ?case by simp
+next
+  case (eva_get cd pc r r' mem ps b act)
+  hence "disassemble cd ! pc = LOD (register_map r) (register_map r')" by simp
   hence "disassemble cd \<tturnstile> MS (inv_register_map ps act) (unmap_mem mem) (Suc pc) \<leadsto>\<^sub>m
-    MS ((inv_register_map ps act)(R5 := (unmap_mem mem) ((inv_register_map ps act) 
-      (register_map r)))) (unmap_mem mem) pc" by (metis evm_lod)
-  with eva_get(2, 3) show ?case by simp
+    MS ((inv_register_map ps act)(register_map r := (unmap_mem mem) ((inv_register_map ps act) 
+      (register_map r')))) (unmap_mem mem) pc" by (metis evm_lod)
+  with eva_get(2, 3, 4) show ?case by simp
 next
   case (eva_puta cd pc r mem ps act)
   hence "disassemble cd ! pc = STO (register_map r) R5" by simp
@@ -359,17 +416,17 @@ theorem correctm_iter [simp]: "iter (\<tturnstile> cd\<^sub>a \<leadsto>\<^sub>a
     iter (\<tturnstile> disassemble cd\<^sub>a \<leadsto>\<^sub>m) (disassemble_state \<Sigma>\<^sub>a) (disassemble_state \<Sigma>\<^sub>a')"
   by (induction \<Sigma>\<^sub>a \<Sigma>\<^sub>a' rule: iter.induct) (simp, metis correctm iter_append iter_one)
 
-lemma [simp]: "inv_register_map (case_register 0 0 0 2 0) Acc = case_reg 0 1 2 11 0" 
+lemma [simp]: "inv_register_map (case_memseg 0 0 0 2 0) Acc = case_reg 0 1 2 11 0" 
   by (auto split: reg.splits)
 
-lemma [simp]: "inv_register_map (case_register hp ep (Suc 0) 0 0) Acc = 
+lemma [simp]: "inv_register_map (case_memseg hp ep (Suc 0) 0 0) Acc = 
     case_reg (4 * hp) (Suc (4 * ep)) 6 3 0"
   by (auto split: reg.splits)
 
 lemma [dest]: "unmap_mem' x = (r, y) \<Longrightarrow> x = 4 * y + register_offset r"
   by (induction x arbitrary: y rule: unmap_mem'.induct) (simp_all split: prod.splits)
 
-lemma [simp]: "unmap_mem (case_register (\<lambda>x. (Acc, 0)) (\<lambda>x. (Acc, 0)) (\<lambda>x. (Acc, 0)) 
+lemma [simp]: "unmap_mem (case_memseg (\<lambda>x. (Acc, 0)) (\<lambda>x. (Acc, 0)) (\<lambda>x. (Acc, 0)) 
   ((\<lambda>x. (Acc, 0)) (0 := (Acc, 0), Suc 0 := (Env, 0))) undefined) = (\<lambda>x. 0)(7 := 1)"
 proof (rule, unfold unmap_mem_def)
   fix x
@@ -381,7 +438,7 @@ proof (rule, unfold unmap_mem_def)
       | _ \<Rightarrow> (\<lambda>x. (Acc, 0))) p) = ((\<lambda>x. 0)(3 := 0, 7 := 1)) x" 
     by (induction r) (simp_all, presburger+, auto)
   with R show "(case unmap_mem' x of (r, p) \<Rightarrow> 
-    pseudoreg_map (case_register (\<lambda>x. (Acc, 0)) (\<lambda>x. (Acc, 0)) (\<lambda>x. (Acc, 0))
+    pseudoreg_map (case_memseg (\<lambda>x. (Acc, 0)) (\<lambda>x. (Acc, 0)) (\<lambda>x. (Acc, 0))
       ((\<lambda>x. (Acc, 0))(0 := (Acc, 0), Suc 0 := (Env, 0))) undefined r p)) =
         ((\<lambda>x. 0)(7 := 1)) x" by simp
 qed
