Readme.md
@@ -20,3 +20,4 @@ Refactorings:
 - Make late stage closures (post bytecode) a single parametric datatype?
 - Clean up isabelle - declare x.simps[intros], assumes/shows, patterns in pfs
 - Use ints insted of nats for machine code
+- Flip environment layout
